Verified alignment for DP-GD

DP-GD_Variant1.dfy
@@ -1,7 +1,7 @@
 // In this variant of DP-GD, we add noise to the summation gradient instead of adding noise to gradient of each sample point
 method DPGD_SummationGradientPerturbation (size:int, learning_rate:real, noise_scale:real, gradient_norm_bound:real, iterations:int) returns (Para:real, PrivacyLost:real)
   requires iterations>=0
-  requires size>=0
+  requires size>0
   requires noise_scale >= 1.0
   requires -1.0 <= gradient_norm_bound <= 1.0
 {
@@ -18,19 +18,35 @@ method DPGD_SummationGradientPerturbation (size:int, learning_rate:real, noise_s
     var i :int := 0;
     var beta:real := 0.0;
     var summation_gradient:real := 0.0;
+    var gradient_alignment:array<real> :=  new real[size];
+    assume gradient_alignment.Length == size;
+    var summation_gradient_alignement:real := sum(gradient_alignment[..1]);
+    assume forall i:int | 0 <= i < gradient_alignment.Length :: (-1.0 <= gradient_alignment[i] <= 1.0);
+    assume forall i:int | 0 <= i <  gradient_alignment.Length :: gradient_alignment[i] != 0.0 ==> (forall j:int | 0 <= j <  gradient_alignment.Length && j != i :: gradient_alignment[j] == 0.0);
     while (i< size)
       invariant i <= size
+      invariant i < size ==> -1.0 <= gradient_alignment[i] <= 1.0
+      invariant i < size ==>  gradient_alignment[i] != 0.0 ==> (forall j:int | 0 <= j <  gradient_alignment.Length && j != i :: gradient_alignment[j] == 0.0)
+      invariant i > 0 ==> summation_gradient_alignement == sum(gradient_alignment[..i])
     {
       var gradient:real := *;
-      // Note: We do not need to clip the value of the gradient.
-      // Instead, we clip the sensitivity of the gradient by the gradient_norm_bound provided by the user
+      gradient_alignment[i] := *; 
+      assume forall i:int | 0 <= i < gradient_alignment.Length :: (-1.0 <= gradient_alignment[i] <= 1.0);
+      assume forall i:int | 0 <= i <  gradient_alignment.Length :: gradient_alignment[i] != 0.0 ==> (forall j:int | 0 <= j <  gradient_alignment.Length && j != i :: gradient_alignment[j] == 0.0);
       summation_gradient := summation_gradient + gradient;
+      summation_gradient_alignement := sum(gradient_alignment[..i+1]);
       i := i + 1;
     }
+    assert summation_gradient_alignement == sum(gradient_alignment[..size]);
+    assert gradient_alignment[..size] == gradient_alignment[..];
+    assert summation_gradient_alignement == sum(gradient_alignment[..]);
+    assume -1.0 <= sum(gradient_alignment[..]) <= 1.0; 
+    assert -1.0 <= summation_gradient_alignement <= 1.0; 
     var eta:real := *;
-    var eta_hat:real := - gradient_norm_bound;
-    assert (gradient_norm_bound + eta_hat == 0.0);
+    var eta_hat:real := - summation_gradient_alignement;
+    assert (summation_gradient_alignement + eta_hat == 0.0);
     summation_gradient := summation_gradient + eta;
+    summation_gradient_alignement := summation_gradient_alignement + eta_hat;
     alpha := alpha + tau;
     thetha[t+1] := thetha[t] - learning_rate*summation_gradient;
     t := t+1;
@@ -41,3 +57,11 @@ method DPGD_SummationGradientPerturbation (size:int, learning_rate:real, noise_s
   PrivacyLost := alpha;
 }
 
+function sum(a:seq<real>) : real
+requires |a| > 0
+{
+  if |a| == 1 then
+    a[0]
+  else
+    a[0] + sum(a[1..])
+}
